
\sigma = \sqrt{\frac 1 n \sum_{i=1}^n (\mu - x_i)^2}

\left.\int_a^b f(x) dx =  F(x) \right\mid_a^b

\lim_{b\to\infty}\int_0^{b}e^{-x^2} dx = \frac{\sqrt{\pi}}{2}

\int_{\int_a^b f(x) dx}^{\int_c^d g(x) dx}h(x)dx

\Gamma(t) = \int_0^{+\infty} x^{t-1}e^{-x}\mathrm{d}\!x = \frac 1 t \prod_{n=1}^{\infty}\frac{(1+\frac 1 t)^t}{1+\frac 1 t} \sim\sqrt{\frac{2\pi}{t}}{\left(\frac t e \right)^t}

\int_0^1 x^x\,\mathrm{d}x = \sum_{n = 1}^\infty{(-1)^{n + 1}\,n^{-n}}

\sideset{_{{}_\alpha^\beta\mathfrak{A}_\delta^\gamma}^{{}_\epsilon^\zeta\mathfrak{B}_\theta^\eta}}{_{{}_\rho^\sigma\mathfrak{E}_\upsilon^\tau}^{{}_\nu^\xi\mathfrak{D}_\pi^o}}\prod_{{}_\phi^\chi\mathfrak{F}_\omega^\psi}^{{}_\iota^\kappa\mathfrak{C}_\mu^\lambda}

\sum_{\substack{1\lt i\lt 3 \\ 1\le j\lt 5}}a_{ij}=\prod^{\substack{1\lt i\lt 3 \\ 1\le j\lt 5}}b_{ij}

\lim_{x\to a} \quad \lim\limits_{x\to a} \quad \int_a^b f(x) dx \quad \int\limits_a^b f(x) dx \quad \sum_{i=0}^n a_i
\quad \sum\limits_{i=0}^n a_i
